<http://vocab.linkeddata.es/datosabiertos/def/medio-ambiente/contaminacion-acustica#hasUnitOfMeasure> <http://www.w3.org/2000/01/rdf-schema#label> "has unit of measure"@en .
<http://vocab.linkeddata.es/datosabiertos/def/medio-ambiente/contaminacion-acustica#hasUnitOfMeasure> <http://www.w3.org/2000/01/rdf-schema#range> <http://www.wurvoc.org/vocabularies/om-1.8/Unit_of_measure> .
<http://vocab.linkeddata.es/datosabiertos/def/medio-ambiente/contaminacion-acustica#hasUnitOfMeasure> <http://www.w3.org/2000/01/rdf-schema#domain> <http://purl.oclc.org/NET/ssnx/ssn#SensorOutput> .
<http://vocab.linkeddata.es/datosabiertos/def/medio-ambiente/contaminacion-acustica#hasUnitOfMeasure> <http://www.w3.org/1999/02/22-rdf-syntax-ns#type> <http://www.w3.org/2002/07/owl#ObjectProperty> .
<http://www.w3.org/2003/01/geo/wgs84_pos#lat_long> <http://www.w3.org/2000/01/rdf-schema#label> "lat/long" .
<http://www.w3.org/2003/01/geo/wgs84_pos#lat_long> <http://www.w3.org/2000/01/rdf-schema#comment> "A comma-separated representation of a latitude, longitude coordinate." .
<http://www.w3.org/2003/01/geo/wgs84_pos#long> <http://www.w3.org/2000/01/rdf-schema#label> "longitude" .
<http://www.w3.org/2003/01/geo/wgs84_pos#long> <http://www.w3.org/2000/01/rdf-schema#label> "longitud"@es .
<http://www.w3.org/2003/01/geo/wgs84_pos#long> <http://www.w3.org/2000/01/rdf-schema#comment> "The WGS84 longitude of a SpatialThing (decimal degrees)." .
<http://www.w3.org/2003/01/geo/wgs84_pos#long> <http://www.w3.org/2000/01/rdf-schema#domain> <http://www.w3.org/2003/01/geo/wgs84_pos#SpatialThing> .
<http://www.w3.org/2003/01/geo/wgs84_pos#long> <http://www.w3.org/1999/02/22-rdf-syntax-ns#type> <http://www.w3.org/2002/07/owl#ObjectProperty> .
<http://www.w3.org/2004/02/skos/core#Concept> <http://www.w3.org/1999/02/22-rdf-syntax-ns#type> <http://www.w3.org/2002/07/owl#Class> .
<http://vocab.linkeddata.es/datosabiertos/def/medio-ambiente/contaminacion-acustica> <http://creativecommons.org/ns#license> "http://creativecommons.org/licenses/by/4.0/" .
<http://vocab.linkeddata.es/datosabiertos/def/medio-ambiente/contaminacion-acustica> <http://purl.org/dc/elements/1.1/rights> "Creative Commons Attribution 4.0 International (CC BY 4.0)" .
<http://vocab.linkeddata.es/datosabiertos/def/medio-ambiente/contaminacion-acustica> <http://purl.org/dc/elements/1.1/title> "Ontolog\u00EDa para Contaminaci\u00F3n Ac\u00FAstica"@es .
<http://vocab.linkeddata.es/datosabiertos/def/medio-ambiente/contaminacion-acustica> <http://purl.org/dc/elements/1.1/description> "Este vocabulario extiende la W3C Semantic Sensor Network Ontology (SSN) con propiedades para representar los datos de la contaminaci\u00F3n ac\u00FAstica. Tambi\u00E9n se extiende la OWL Ontology of Time (OWL-Time)  para representar el tiempo y la WGS84 Geo Positioning para representar la posici\u00F3n en el espacio a trav\u00E9s de la longitud, latitud y altitud"@es .
<http://vocab.linkeddata.es/datosabiertos/def/medio-ambiente/contaminacion-acustica> <http://www.w3.org/2002/07/owl#imports> <http://www.w3.org/2006/time> .
<http://vocab.linkeddata.es/datosabiertos/def/medio-ambiente/contaminacion-acustica> <http://www.w3.org/2002/07/owl#imports> <http://purl.oclc.org/NET/ssnx/ssn> .
<http://vocab.linkeddata.es/datosabiertos/def/medio-ambiente/contaminacion-acustica> <http://www.w3.org/1999/02/22-rdf-syntax-ns#type> <http://www.w3.org/2002/07/owl#Ontology> .
<http://www.w3.org/2003/01/geo/wgs84_pos#SpatialThing> <http://www.w3.org/2000/01/rdf-schema#label> "SpatialThing" .
<http://www.w3.org/2003/01/geo/wgs84_pos#SpatialThing> <http://www.w3.org/2000/01/rdf-schema#comment> "Anything with spatial extent, i.e. size, shape, or position.\n e.g. people, places, bowling balls, as well as abstract areas like cubes.\n" .
<http://www.w3.org/2003/01/geo/wgs84_pos#SpatialThing> <http://www.w3.org/1999/02/22-rdf-syntax-ns#type> <http://www.w3.org/2002/07/owl#Class> .
<http://www.w3.org/2003/01/geo/wgs84_pos#> <http://purl.org/dc/elements/1.1/title> "WGS84 Geo Positioning: an RDF vocabulary" .
<http://www.w3.org/2003/01/geo/wgs84_pos#> <http://www.w3.org/2000/01/rdf-schema#comment> "\nRecent changes to this namespace:\n$Log: wgs84_pos.rdf,v $\nRevision 1.22  2009/04/20 15:00:30  timbl\nRemove the time bits which have been deal with elsewhere eg in iCal.\n\nRevision 1.21  2009/04/20 12:52:47  timbl\ntry again\n\nRevision 1.20  2009/04/20 12:42:11  timbl\nAdd Event (edited ages ago and never checked in), and location (following discussion http://chatlogs.planetrdf.com/swig/2009-04-20#T12-36-09)\n\nRevision 1.19  2009/04/20 12:36:31  timbl\nAdd Event (edited ages ago and never checked in), and location (following discussion http://chatlogs.planetrdf.com/swig/2009-04-20#T12-36-09)\n\nRevision 1.18  2006/02/01 22:01:04  danbri\nClarified that lat and long are decimal degrees, and that alt is decimal metres about local reference ellipsoid\n\nRevision 1.17  2004/02/06 17:38:12  danbri\nFixed a bad commit screwup\n\nRevision 1.15  2003/04/19 11:24:08  danbri\nFixed the typo even more.\n\nRevision 1.14  2003/04/19 11:16:56  danbri\nfixed a typo\n\nRevision 1.13  2003/02/19 22:27:27  connolly\nrelaxed domain constraints on lat/long/alt from Point to SpatialThing\n\nRevision 1.12  2003/01/12 01:41:41  danbri\nTrying local copy of XSLT doc.\n\nRevision 1.11  2003/01/12 01:20:18  danbri\nadded a link to morten's xslt rdfs viewer.\n\nRevision 1.10  2003/01/11 18:56:49  danbri\nRemoved datatype range from lat and long properties, since they would\nhave required each occurance of the property to mention the datatype.\n\nRevision 1.9  2003/01/11 11:41:31  danbri\nAnother typo; repaired rdfs:Property to rdf:Property x4\n\nRevision 1.8  2003/01/11 11:05:02  danbri\nAdded an rdfs:range for each lat/long/alt property,\nhttp://www.w3.org/2001/XMLSchema#float\n\nRevision 1.7  2003/01/10 20:25:16  danbri\nLonger rdfs:comment for Point, trying to be Earth-centric and neutral about\ncoordinate system(s) at the same time. Feedback welcomed.\n\nRevision 1.6  2003/01/10 20:18:30  danbri\nAdded CVS log comments into the RDF/XML as an rdfs:comment property of the\nvocabulary. Note that this is not common practice (but seems both harmless\nand potentially useful).\n\n\nrevision 1.5\ndate: 2003/01/10 20:14:31;  author: danbri;  state: Exp;  lines: +16 -5\nUpdated schema:\nAdded a dc:date, added url for more info. Changed the rdfs:label of the\nnamespace from gp to geo. Added a class Point, set as the rdfs:domain of\neach property. Added XML comment on the lat_long property suggesting that\nwe might not need it (based on #rdfig commentary from implementors).\n\nrevision 1.4\ndate: 2003/01/10 20:01:07;  author: danbri;  state: Exp;  lines: +6 -5\nFixed typo; several rdfs:about attributes are now rdf:about. Thanks to MortenF in\n#rdfig for catching this error.\n\nrevision 1.3\ndate: 2003/01/10 11:59:03;  author: danbri;  state: Exp;  lines: +4 -3\nfixed buglet in vocab, added more wgs links\n\nrevision 1.2\ndate: 2003/01/10 11:01:11;  author: danbri;  state: Exp;  lines: +4 -4\nRemoved alt from the as-a-flat-string property, and switched from\nspace separated to comma separated.\n\nrevision 1.1\ndate: 2003/01/10 10:53:23;  author: danbri;  state: Exp;\nbasic geo vocab\n\n" .
<http://www.w3.org/2003/01/geo/wgs84_pos#> <http://purl.org/dc/elements/1.1/description> "A vocabulary for representing latitude, longitude and \n altitude information in the WGS84 geodetic reference datum. \n Version $Id: wgs84_pos.rdf,v 1.22 2009/04/20 15:00:30 timbl Exp $. See http://www.w3.org/2003/01/geo/ for more details." .
<http://www.w3.org/2003/01/geo/wgs84_pos#> <http://www.w3.org/2000/01/rdf-schema#label> "geo" .
<http://www.w3.org/2003/01/geo/wgs84_pos#> <http://purl.org/dc/elements/1.1/date> "$Date: 2009/04/20 15:00:30 $" .
<http://vocab.linkeddata.es/datosabiertos/def/medio-ambiente/contaminacion-acustica#ClaseII> <http://www.w3.org/2000/01/rdf-schema#seeAlso> "Normativa internacional IEC 61672-1:2013"@es .
<http://vocab.linkeddata.es/datosabiertos/def/medio-ambiente/contaminacion-acustica#ClaseII> <http://www.w3.org/2000/01/rdf-schema#label> "Clase II"@es .
<http://vocab.linkeddata.es/datosabiertos/def/medio-ambiente/contaminacion-acustica#ClaseII> <http://www.w3.org/2000/01/rdf-schema#comment> "Sensor que cumple las caracter\u00EDsticas de precisi\u00F3n menos restrictivas definidas en la normativa IEC. Esta clase de sensores tiene mayores m\u00E1rgenes de tolerancia en su rango de medida."@es .
<http://vocab.linkeddata.es/datosabiertos/def/medio-ambiente/contaminacion-acustica#ClaseII> <http://www.w3.org/1999/02/22-rdf-syntax-ns#type> <http://www.w3.org/2004/02/skos/core#Concept> .
<http://vocab.linkeddata.es/datosabiertos/def/medio-ambiente/contaminacion-acustica#ClaseII> <http://www.w3.org/1999/02/22-rdf-syntax-ns#type> <http://www.w3.org/2002/07/owl#NamedIndividual> .
<http://purl.oclc.org/NET/ssnx/ssn#observationSamplingTime> <http://www.w3.org/2000/01/rdf-schema#range> <http://www.w3.org/2006/time#TemporalEntity> .
<http://purl.oclc.org/NET/ssnx/ssn#observationSamplingTime> <http://www.w3.org/2000/01/rdf-schema#domain> <http://purl.oclc.org/NET/ssnx/ssn#ObservationValue> .
<http://vocab.linkeddata.es/datosabiertos/def/medio-ambiente/contaminacion-acustica#NoiseSensor> <http://www.w3.org/2000/01/rdf-schema#label> "Sensor de Ruido"@es .
<http://vocab.linkeddata.es/datosabiertos/def/medio-ambiente/contaminacion-acustica#NoiseSensor> <http://www.w3.org/2000/01/rdf-schema#label> "Noise Sensor"@en .
<http://vocab.linkeddata.es/datosabiertos/def/medio-ambiente/contaminacion-acustica#NoiseSensor> <http://www.w3.org/2000/01/rdf-schema#comment> "Mide el nivel de ruido"@es .
<http://vocab.linkeddata.es/datosabiertos/def/medio-ambiente/contaminacion-acustica#NoiseSensor> <http://www.w3.org/2000/01/rdf-schema#subClassOf> <http://purl.oclc.org/NET/ssnx/ssn#SensingDevice> .
<http://vocab.linkeddata.es/datosabiertos/def/medio-ambiente/contaminacion-acustica#NoiseSensor> <http://www.w3.org/1999/02/22-rdf-syntax-ns#type> <http://www.w3.org/2002/07/owl#Class> .
<http://vocab.linkeddata.es/datosabiertos/def/medio-ambiente/contaminacion-acustica#AverageNoiseLevel> <http://www.w3.org/2000/01/rdf-schema#label> "Nivel Medio de Ruido"@es .
<http://vocab.linkeddata.es/datosabiertos/def/medio-ambiente/contaminacion-acustica#AverageNoiseLevel> <http://www.w3.org/2000/01/rdf-schema#label> "Average Noise Level"@en .
<http://vocab.linkeddata.es/datosabiertos/def/medio-ambiente/contaminacion-acustica#AverageNoiseLevel> <http://www.w3.org/2000/01/rdf-schema#comment> "Nivel medio de ruido que ha sido medido por el sensor."@es .
<http://vocab.linkeddata.es/datosabiertos/def/medio-ambiente/contaminacion-acustica#AverageNoiseLevel> <http://www.w3.org/2000/01/rdf-schema#subClassOf> <http://purl.oclc.org/NET/ssnx/ssn#Property> .
<http://vocab.linkeddata.es/datosabiertos/def/medio-ambiente/contaminacion-acustica#AverageNoiseLevel> <http://www.w3.org/1999/02/22-rdf-syntax-ns#type> <http://www.w3.org/2002/07/owl#Class> .
<http://vocab.linkeddata.es/datosabiertos/def/medio-ambiente/contaminacion-acustica#PonderacionC> <http://www.w3.org/2000/01/rdf-schema#seeAlso> "Norma IEC 61672:2003"@es .
<http://vocab.linkeddata.es/datosabiertos/def/medio-ambiente/contaminacion-acustica#PonderacionC> <http://www.w3.org/2000/01/rdf-schema#label> "Ponderaci\u00F3n C"@es .
<http://vocab.linkeddata.es/datosabiertos/def/medio-ambiente/contaminacion-acustica#PonderacionC> <http://www.w3.org/2000/01/rdf-schema#comment> "Ponderaci\u00F3n que se utiliza para evaluar altos niveles de ruido."@es .
<http://vocab.linkeddata.es/datosabiertos/def/medio-ambiente/contaminacion-acustica#PonderacionC> <http://www.w3.org/1999/02/22-rdf-syntax-ns#type> <http://www.w3.org/2004/02/skos/core#Concept> .
<http://vocab.linkeddata.es/datosabiertos/def/medio-ambiente/contaminacion-acustica#PonderacionC> <http://www.w3.org/1999/02/22-rdf-syntax-ns#type> <http://vocab.linkeddata.es/datosabiertos/def/medio-ambiente/contaminacion-acustica#Weighting> .
<http://vocab.linkeddata.es/datosabiertos/def/medio-ambiente/contaminacion-acustica#PonderacionC> <http://www.w3.org/1999/02/22-rdf-syntax-ns#type> <http://www.w3.org/2002/07/owl#NamedIndividual> .
<http://www.w3.org/2003/01/geo/wgs84_pos#alt> <http://www.w3.org/2000/01/rdf-schema#label> "altitude" .
<http://www.w3.org/2003/01/geo/wgs84_pos#alt> <http://www.w3.org/2000/01/rdf-schema#label> "altitud"@es .
<http://www.w3.org/2003/01/geo/wgs84_pos#alt> <http://www.w3.org/2000/01/rdf-schema#comment> "The WGS84 altitude of a SpatialThing (decimal meters \nabove the local reference ellipsoid)." .
<http://www.w3.org/2003/01/geo/wgs84_pos#alt> <http://www.w3.org/2000/01/rdf-schema#domain> <http://www.w3.org/2003/01/geo/wgs84_pos#SpatialThing> .
<http://www.w3.org/2003/01/geo/wgs84_pos#alt> <http://www.w3.org/1999/02/22-rdf-syntax-ns#type> <http://www.w3.org/2002/07/owl#ObjectProperty> .
<http://www.wurvoc.org/vocabularies/om-1.8/Unit_of_measure> <http://www.w3.org/1999/02/22-rdf-syntax-ns#type> <http://www.w3.org/2002/07/owl#Class> .
<http://vocab.linkeddata.es/datosabiertos/def/medio-ambiente/contaminacion-acustica#NoiseLevel> <http://www.w3.org/2000/01/rdf-schema#label> "Noise Level"@en .
<http://vocab.linkeddata.es/datosabiertos/def/medio-ambiente/contaminacion-acustica#NoiseLevel> <http://www.w3.org/2000/01/rdf-schema#label> "Nivel de Ruido"@es .
<http://vocab.linkeddata.es/datosabiertos/def/medio-ambiente/contaminacion-acustica#NoiseLevel> <http://www.w3.org/2000/01/rdf-schema#comment> "Nivel de ruido que ha sido medido por el sensor. Se mide en Decibelios (dB)"@es .
<http://vocab.linkeddata.es/datosabiertos/def/medio-ambiente/contaminacion-acustica#NoiseLevel> <http://www.w3.org/2000/01/rdf-schema#subClassOf> <http://purl.oclc.org/NET/ssnx/ssn#Property> .
<http://vocab.linkeddata.es/datosabiertos/def/medio-ambiente/contaminacion-acustica#NoiseLevel> <http://www.w3.org/1999/02/22-rdf-syntax-ns#type> <http://www.w3.org/2002/07/owl#Class> .
<http://vocab.linkeddata.es/datosabiertos/def/medio-ambiente/contaminacion-acustica#belongsToSensorClass> <http://www.w3.org/2000/01/rdf-schema#label> "pertenece a una Clase de Sensor"@es .
<http://vocab.linkeddata.es/datosabiertos/def/medio-ambiente/contaminacion-acustica#belongsToSensorClass> <http://www.w3.org/2000/01/rdf-schema#label> "belongs to Sensor Class"@en .
<http://vocab.linkeddata.es/datosabiertos/def/medio-ambiente/contaminacion-acustica#belongsToSensorClass> <http://www.w3.org/2000/01/rdf-schema#comment> "Un Sensor tiene unas caracter\u00EDsticas espec\u00EDficas seg\u00FAn la Clase a la que pertenece. Puede ser de Clase I o II o no pertenecer a ninguna Clase."@es .
<http://vocab.linkeddata.es/datosabiertos/def/medio-ambiente/contaminacion-acustica#belongsToSensorClass> <http://www.w3.org/2000/01/rdf-schema#range> <http://www.w3.org/2004/02/skos/core#Concept> .
<http://vocab.linkeddata.es/datosabiertos/def/medio-ambiente/contaminacion-acustica#belongsToSensorClass> <http://www.w3.org/2000/01/rdf-schema#domain> <http://vocab.linkeddata.es/datosabiertos/def/medio-ambiente/contaminacion-acustica#NoiseSensor> .
<http://vocab.linkeddata.es/datosabiertos/def/medio-ambiente/contaminacion-acustica#belongsToSensorClass> <http://www.w3.org/1999/02/22-rdf-syntax-ns#type> <http://www.w3.org/2002/07/owl#ObjectProperty> .
<http://www.w3.org/2003/01/geo/wgs84_pos#Point> <http://www.w3.org/2000/01/rdf-schema#label> "point" .
<http://www.w3.org/2003/01/geo/wgs84_pos#Point> <http://www.w3.org/2000/01/rdf-schema#comment> "A point, typically described using a coordinate system relative to Earth, such as WGS84.\n  " .
<http://www.w3.org/2003/01/geo/wgs84_pos#Point> <http://www.w3.org/2000/01/rdf-schema#comment> " \nUniquely identified by lat/long/alt. i.e.\n\nspaciallyIntersects(P1, P2) :- lat(P1, LAT), long(P1, LONG), alt(P1, ALT),\n  lat(P2, LAT), long(P2, LONG), alt(P2, ALT).\n\nsameThing(P1, P2) :- type(P1, Point), type(P2, Point), spaciallyIntersects(P1, P2).\n  " .
<http://www.w3.org/2003/01/geo/wgs84_pos#Point> <http://www.w3.org/2000/01/rdf-schema#subClassOf> <http://www.w3.org/2003/01/geo/wgs84_pos#SpatialThing> .
<http://www.w3.org/2003/01/geo/wgs84_pos#Point> <http://www.w3.org/1999/02/22-rdf-syntax-ns#type> <http://www.w3.org/2002/07/owl#Class> .
<http://dbpedia.org/resource/Decibel> <http://www.w3.org/1999/02/22-rdf-syntax-ns#type> <http://www.wurvoc.org/vocabularies/om-1.8/Unit_of_measure> .
<http://dbpedia.org/resource/Decibel> <http://www.w3.org/1999/02/22-rdf-syntax-ns#type> <http://www.w3.org/2002/07/owl#NamedIndividual> .
<http://vocab.linkeddata.es/datosabiertos/def/medio-ambiente/contaminacion-acustica#PonderacionZ> <http://www.w3.org/2000/01/rdf-schema#seeAlso> "Norma IEC 61672:2003"@es .
<http://vocab.linkeddata.es/datosabiertos/def/medio-ambiente/contaminacion-acustica#PonderacionZ> <http://www.w3.org/2000/01/rdf-schema#label> "Ponderaci\u00F3n Z"@es .
<http://vocab.linkeddata.es/datosabiertos/def/medio-ambiente/contaminacion-acustica#PonderacionZ> <http://www.w3.org/2000/01/rdf-schema#comment> "Representa el hecho de no aplicar ning\u00FAn tipo de ponderaci\u00F3n frecuencial a las ondas sonoras captadas por el sensor de ruido. Se captan tal y como son."@es .
<http://vocab.linkeddata.es/datosabiertos/def/medio-ambiente/contaminacion-acustica#PonderacionZ> <http://www.w3.org/1999/02/22-rdf-syntax-ns#type> <http://www.w3.org/2004/02/skos/core#Concept> .
<http://vocab.linkeddata.es/datosabiertos/def/medio-ambiente/contaminacion-acustica#PonderacionZ> <http://www.w3.org/1999/02/22-rdf-syntax-ns#type> <http://vocab.linkeddata.es/datosabiertos/def/medio-ambiente/contaminacion-acustica#Weighting> .
<http://vocab.linkeddata.es/datosabiertos/def/medio-ambiente/contaminacion-acustica#PonderacionZ> <http://www.w3.org/1999/02/22-rdf-syntax-ns#type> <http://www.w3.org/2002/07/owl#NamedIndividual> .
<http://vocab.linkeddata.es/datosabiertos/def/medio-ambiente/contaminacion-acustica#ClaseI> <http://www.w3.org/2000/01/rdf-schema#seeAlso> "Normativa internacional IEC 61672-1:2013"@es .
<http://vocab.linkeddata.es/datosabiertos/def/medio-ambiente/contaminacion-acustica#ClaseI> <http://www.w3.org/2000/01/rdf-schema#label> "Clase I"@es .
<http://vocab.linkeddata.es/datosabiertos/def/medio-ambiente/contaminacion-acustica#ClaseI> <http://www.w3.org/2000/01/rdf-schema#comment> "Sensor que cumple las caracter\u00EDsticas de precisi\u00F3n m\u00E1s restrictivas definidas en la normativa IEC. Esta clase de sensores tiene menores m\u00E1rgenes de tolerancia en su rango de medida."@es .
<http://vocab.linkeddata.es/datosabiertos/def/medio-ambiente/contaminacion-acustica#ClaseI> <http://www.w3.org/1999/02/22-rdf-syntax-ns#type> <http://www.w3.org/2004/02/skos/core#Concept> .
<http://vocab.linkeddata.es/datosabiertos/def/medio-ambiente/contaminacion-acustica#ClaseI> <http://www.w3.org/1999/02/22-rdf-syntax-ns#type> <http://www.w3.org/2002/07/owl#NamedIndividual> .
<http://vocab.linkeddata.es/datosabiertos/def/medio-ambiente/contaminacion-acustica#PonderacionA> <http://www.w3.org/2000/01/rdf-schema#seeAlso> "Norma IEC 61672:2003"@es .
<http://vocab.linkeddata.es/datosabiertos/def/medio-ambiente/contaminacion-acustica#PonderacionA> <http://www.w3.org/2000/01/rdf-schema#label> "Ponderaci\u00F3n A"@es .
<http://vocab.linkeddata.es/datosabiertos/def/medio-ambiente/contaminacion-acustica#PonderacionA> <http://www.w3.org/2000/01/rdf-schema#comment> "Ponderaci\u00F3n m\u00E1s habitual en ac\u00FAstica ambiental. Se utiliza para ajustar los niveles de ruido a c\u00F3mo los percibe el oido humano."@es .
<http://vocab.linkeddata.es/datosabiertos/def/medio-ambiente/contaminacion-acustica#PonderacionA> <http://www.w3.org/1999/02/22-rdf-syntax-ns#type> <http://www.w3.org/2004/02/skos/core#Concept> .
<http://vocab.linkeddata.es/datosabiertos/def/medio-ambiente/contaminacion-acustica#PonderacionA> <http://www.w3.org/1999/02/22-rdf-syntax-ns#type> <http://vocab.linkeddata.es/datosabiertos/def/medio-ambiente/contaminacion-acustica#Weighting> .
<http://vocab.linkeddata.es/datosabiertos/def/medio-ambiente/contaminacion-acustica#PonderacionA> <http://www.w3.org/1999/02/22-rdf-syntax-ns#type> <http://www.w3.org/2002/07/owl#NamedIndividual> .
<http://vocab.linkeddata.es/datosabiertos/def/medio-ambiente/contaminacion-acustica#PercentilNoiseLevel> <http://www.w3.org/2000/01/rdf-schema#label> "Nivel de Ruido en Percentiles"@es .
<http://vocab.linkeddata.es/datosabiertos/def/medio-ambiente/contaminacion-acustica#PercentilNoiseLevel> <http://www.w3.org/2000/01/rdf-schema#subClassOf> <http://purl.oclc.org/NET/ssnx/ssn#Property> .
<http://vocab.linkeddata.es/datosabiertos/def/medio-ambiente/contaminacion-acustica#PercentilNoiseLevel> <http://www.w3.org/1999/02/22-rdf-syntax-ns#type> <http://www.w3.org/2002/07/owl#Class> .
<http://vocab.linkeddata.es/datosabiertos/def/medio-ambiente/contaminacion-acustica#lastCalibrationDate> <http://www.w3.org/2000/01/rdf-schema#label> "\u00FAltima fecha de calibraci\u00F3n"@es .
<http://vocab.linkeddata.es/datosabiertos/def/medio-ambiente/contaminacion-acustica#lastCalibrationDate> <http://www.w3.org/2000/01/rdf-schema#label> "last calibration date"@en .
<http://vocab.linkeddata.es/datosabiertos/def/medio-ambiente/contaminacion-acustica#lastCalibrationDate> <http://www.w3.org/2000/01/rdf-schema#comment> "\u00DAltima fecha de calibraci\u00F3n del sensor.  La calibraci\u00F3n es un proceso peri\u00F3dico realizado a los sensores ac\u00FAsticos para verificar su correcto funcionamiento en sus distintos modos de trabajo."@es .
<http://vocab.linkeddata.es/datosabiertos/def/medio-ambiente/contaminacion-acustica#lastCalibrationDate> <http://www.w3.org/2000/01/rdf-schema#range> <http://www.w3.org/2001/XMLSchema#dateTime> .
<http://vocab.linkeddata.es/datosabiertos/def/medio-ambiente/contaminacion-acustica#lastCalibrationDate> <http://www.w3.org/2000/01/rdf-schema#domain> <http://vocab.linkeddata.es/datosabiertos/def/medio-ambiente/contaminacion-acustica#NoiseSensor> .
<http://vocab.linkeddata.es/datosabiertos/def/medio-ambiente/contaminacion-acustica#lastCalibrationDate> <http://www.w3.org/1999/02/22-rdf-syntax-ns#type> <http://www.w3.org/2002/07/owl#DatatypeProperty> .
<http://www.w3.org/2003/01/geo/wgs84_pos#location> <http://www.w3.org/2000/01/rdf-schema#comment> "The relation between something and the point, \n or other geometrical thing in space, where it is.  For example, the realtionship between\n a radio tower and a Point with a given lat and long.\n Or a relationship between a park and its outline as a closed arc of points, or a road and\n its location as a arc (a sequence of points).\n Clearly in practice there will be limit to the accuracy of any such statement, but one would expect\n an accuracy appropriate for the size of the object and uses such as mapping .\n " .
<http://www.w3.org/2003/01/geo/wgs84_pos#location> <http://www.w3.org/2000/01/rdf-schema#label> "location" .
<http://www.w3.org/2003/01/geo/wgs84_pos#location> <http://www.w3.org/2000/01/rdf-schema#domain> <http://purl.oclc.org/NET/ssnx/ssn#SensingDevice> .
<http://www.w3.org/2003/01/geo/wgs84_pos#location> <http://www.w3.org/1999/02/22-rdf-syntax-ns#type> <http://www.w3.org/2002/07/owl#ObjectProperty> .
<http://www.w3.org/2003/01/geo/wgs84_pos#location> <http://www.w3.org/2000/01/rdf-schema#range> <http://www.w3.org/2003/01/geo/wgs84_pos#SpatialThing> .
<http://www.w3.org/2003/01/geo/wgs84_pos#location> <http://www.w3.org/2000/01/rdf-schema#subPropertyOf> <http://xmlns.com/foaf/0.1/based_near> .
<http://www.w3.org/2003/01/geo/wgs84_pos#location> <http://www.w3.org/1999/02/22-rdf-syntax-ns#type> <http://www.w3.org/2002/07/owl#AnnotationProperty> .
<http://purl.org/dc/elements/1.1/description> <http://www.w3.org/1999/02/22-rdf-syntax-ns#type> <http://www.w3.org/2002/07/owl#AnnotationProperty> .
<http://purl.org/vocab/vann/preferredNamespaceUri> <http://www.w3.org/1999/02/22-rdf-syntax-ns#type> <http://www.w3.org/2002/07/owl#AnnotationProperty> .
<http://vocab.linkeddata.es/datosabiertos/def/medio-ambiente/contaminacion-acustica#Weighting> <http://www.w3.org/2000/01/rdf-schema#label> "Weighting"@en .
<http://vocab.linkeddata.es/datosabiertos/def/medio-ambiente/contaminacion-acustica#Weighting> <http://www.w3.org/2000/01/rdf-schema#label> "Ponderaci\u00F3n"@es .
<http://vocab.linkeddata.es/datosabiertos/def/medio-ambiente/contaminacion-acustica#Weighting> <http://www.w3.org/2000/01/rdf-schema#comment> "La medida que realiza el Sensor de Ruido tiene una ponderaci\u00F3n frecuencial. Puede ser sin poderaci\u00F3n (Z), ponderaci\u00F3n A o C"@es .
<http://vocab.linkeddata.es/datosabiertos/def/medio-ambiente/contaminacion-acustica#Weighting> <http://www.w3.org/2000/01/rdf-schema#subClassOf> <http://www.loa-cnr.it/ontologies/DUL.owl#Method> .
<http://vocab.linkeddata.es/datosabiertos/def/medio-ambiente/contaminacion-acustica#Weighting> <http://www.w3.org/1999/02/22-rdf-syntax-ns#type> <http://www.w3.org/2002/07/owl#Class> .
<http://www.w3.org/2003/01/geo/wgs84_pos#lat> <http://www.w3.org/2000/01/rdf-schema#label> "latitude" .
<http://www.w3.org/2003/01/geo/wgs84_pos#lat> <http://www.w3.org/2000/01/rdf-schema#label> "latitud"@es .
<http://www.w3.org/2003/01/geo/wgs84_pos#lat> <http://www.w3.org/2000/01/rdf-schema#comment> "The WGS84 latitude of a SpatialThing (decimal degrees)." .
<http://www.w3.org/2003/01/geo/wgs84_pos#lat> <http://www.w3.org/2000/01/rdf-schema#domain> <http://www.w3.org/2003/01/geo/wgs84_pos#SpatialThing> .
<http://www.w3.org/2003/01/geo/wgs84_pos#lat> <http://www.w3.org/1999/02/22-rdf-syntax-ns#type> <http://www.w3.org/2002/07/owl#ObjectProperty> .
<http://vocab.linkeddata.es/datosabiertos/def/medio-ambiente/contaminacion-acustica#isWeightingWith> <http://www.w3.org/2000/01/rdf-schema#label> "is weightin with"@en .
<http://vocab.linkeddata.es/datosabiertos/def/medio-ambiente/contaminacion-acustica#isWeightingWith> <http://www.w3.org/2000/01/rdf-schema#label> "es ponderado con"@es .
<http://vocab.linkeddata.es/datosabiertos/def/medio-ambiente/contaminacion-acustica#isWeightingWith> <http://www.w3.org/2000/01/rdf-schema#comment> "La medida que realiza el Sensor de Ruido tiene una ponderaci\u00F3n frecuencial. Puede ser sin poderaci\u00F3n (Z), ponderaci\u00F3n A o C"@es .
<http://vocab.linkeddata.es/datosabiertos/def/medio-ambiente/contaminacion-acustica#isWeightingWith> <http://www.w3.org/2000/01/rdf-schema#range> <http://vocab.linkeddata.es/datosabiertos/def/medio-ambiente/contaminacion-acustica#Weighting> .
<http://vocab.linkeddata.es/datosabiertos/def/medio-ambiente/contaminacion-acustica#isWeightingWith> <http://www.w3.org/2000/01/rdf-schema#domain> <http://purl.oclc.org/NET/ssnx/ssn#ObservationValue> .
<http://vocab.linkeddata.es/datosabiertos/def/medio-ambiente/contaminacion-acustica#isWeightingWith> <http://www.w3.org/1999/02/22-rdf-syntax-ns#type> <http://www.w3.org/2002/07/owl#ObjectProperty> .
<http://xmlns.com/foaf/0.1/based_near> <http://www.w3.org/1999/02/22-rdf-syntax-ns#type> <http://www.w3.org/2002/07/owl#AnnotationProperty> .
<http://purl.org/vocab/vann/preferredNamespacePrefix> <http://www.w3.org/1999/02/22-rdf-syntax-ns#type> <http://www.w3.org/2002/07/owl#AnnotationProperty> .
